xv6-RISCV-impl/kernel/kalloc.c
@@ -15,17 +15,18 @@ extern char end[]; // first address after kernel.
                    // defined by kernel.ld.
 
 struct run {
-  struct run *next; 
+  struct run *next;
 };
 
-// kmem is now a single instance of this struct, allocated in global memory.
 struct {
+  struct spinlock lock;
   struct run *freelist;
 } kmem;
 
 void
 kinit()
 {
+  initlock(&kmem.lock, "kmem");
   freerange(end, (void*)PHYSTOP);
 }
 
@@ -43,27 +44,39 @@ freerange(void *pa_start, void *pa_end)
 // call to kalloc().  (The exception is when
 // initializing the allocator; see kinit above.)
 void
-kfree(void *pa) // LINE: kind of add ( push)
+kfree(void *pa)
 {
   struct run *r;
 
+  if(((uint64)pa % PGSIZE) != 0 || (char*)pa < end || (uint64)pa >= PHYSTOP)
+    panic("kfree");
+
+  // Fill with junk to catch dangling refs.
+  memset(pa, 1, PGSIZE);
+
   r = (struct run*)pa;
 
+  acquire(&kmem.lock);
   r->next = kmem.freelist;
   kmem.freelist = r;
+  release(&kmem.lock);
 }
 
 // Allocate one 4096-byte page of physical memory.
 // Returns a pointer that the kernel can use.
 // Returns 0 if the memory cannot be allocated.
 void *
-kalloc(void) // LINE: kind of remove / pop
+kalloc(void)
 {
   struct run *r;
 
+  acquire(&kmem.lock);
   r = kmem.freelist;
   if(r)
     kmem.freelist = r->next;
+  release(&kmem.lock);
 
-  return (void*)r;
+  if(r)
+    memset((char*)r, 5, PGSIZE); // fill with junk
+  return (void*)r; 
 }
