VST-introduction/VSU_client1_fromVC.v
@@ -18,7 +18,7 @@ Definition t_run := Tstruct _run noattr.
 Fixpoint freelistrep (sh: share) (n: nat) (p: val) : mpred :=
  match n with
  | S n' => EX next: val, 
-        !! malloc_compatible (sizeof t_run) p &&  (* p is compatible with a memory block of size sizeof theader. *)
+        !! malloc_compatible (PGSIZE) p &&  (* p is compatible with a memory block of size sizeof theader. *)
         data_at sh t_run next p * (* at the location p, there is a t_run structure with the value next *)
         freelistrep sh n' next (* "*" ensures no loops... *)
  | O => !! (p = nullval) && emp
@@ -68,7 +68,7 @@ Lemma freelistrep_nonnull: forall n sh x,
    x <> nullval ->
    freelistrep sh n x =
    EX m : nat, EX next:val,
-          !! (n = S m) && !! malloc_compatible (sizeof t_run) x && data_at sh t_run next x * freelistrep sh m next.
+          !! (n = S m) && !! malloc_compatible (PGSIZE) x && data_at sh t_run next x * freelistrep sh m next.
 Proof.
    intros; apply pred_ext.
    - destruct n. 
@@ -83,7 +83,7 @@ Qed.
  
 Definition malloc_token_sz (sh: share) (n: Z) (p: val) : mpred := 
   !! (field_compatible t_run [] p 
-      /\ malloc_compatible (sizeof t_run) p
+      /\ malloc_compatible (PGSIZE) p
       /\ 0 <= n <= sizeof t_run) 
  &&  memory_block Ews (sizeof t_run - n) (offset_val n p).
 
